# 参考系变换

## 直角坐标系

设有参考系$S(i,j,k)$与$S'(i',j',k')$,间距$r_0$

对$S'$系坐标基矢求绝对微商可得:
$$
\frac{D\vec {i'}}{Dt}=\vec\omega\times\vec {i'},~~~\frac{D\vec {j'}}{Dt}=\vec\omega\times\vec {j'},~~~\frac{D\vec {k'}}{Dt}=\vec\omega\times\vec {k'}
$$
此处的$\vec\omega$指$S'$系的角速度

对$\vec {a'}=(x'\vec {i'}+y'\vec{j'}+z'\vec{k'})$求绝对微商可得:
$$
\begin{aligned}
\frac{Da'}{Dt}&=\frac D{Dt}(x'\vec {i'}+y'\vec{j'}+z'\vec{k'})\\
&=\frac{Dx'}{Dt}\vec{i'}+\frac{Dy'}{Dt}\vec{j'}+\frac{Dz'}{Dt}\vec{k'}+x'\frac{D\vec{i'}}{Dt}+y'\frac{D\vec{j'}}{Dt}+z'\frac{D\vec{k'}}{Dt}\\
&=\frac{dx'}{dt}\vec{i'}+\frac{dy'}{dt}\vec{j'}+\frac{dz'}{dt}\vec{k'}+x'\vec\omega\times \vec{i'}+y'\vec\omega\times \vec{j'}+z'\vec\omega\times \vec{k'}\\
&=\frac d{dt}(x'\vec {i'}+y'\vec{j'}+z'\vec{k'})+\vec\omega\times(x'\vec {i'}+y'\vec{j'}+z'\vec{k'})\\
&=\frac{d\vec{a'}}{dt}+\vec\omega\times\vec{a'}
\end{aligned}
$$
由:
$$
\vec r=\vec{r_0}+\vec{r'}
$$

$$
\begin{aligned}
v=\frac{D\vec r}{Dt}&=\frac{D\vec{r_0}}{Dt}+\frac{D\vec{r'}}{Dt}\\
&=\frac{D\vec{r_0}}{Dt}+\frac{d\vec{r'}}{dt}+\vec\omega\times\vec{r'}\\
&=\vec{v_0}+\vec{v'}+\vec\omega\times\vec{r'}
\end{aligned}
$$

则:
$$
\begin{aligned}
\vec a=\frac{D\vec v}{Dt}&=\frac{D}{Dt}(\vec{v_0}+\vec{v'}+\vec\omega\times\vec{r'})\\
&=\vec{a_0}+\frac{d\vec{v'}}{dt}+\vec\omega\times\vec{v'}+\vec\alpha\times\vec{r'}+\vec\omega\times(\vec{v'}+\vec\omega\times\vec{r'})\\
&=\vec{a_0}+\vec{a'}+2\vec\omega\times\vec{v'}+\vec\alpha\times\vec{r'}+\vec\omega\times(\vec\omega\times\vec{r'})
\end{aligned}
$$

## 极坐标系

设有参考系$S(r,\theta),S'(r',\theta')$,间距$\theta_0$

对矢量$\vec {a}=a\cdot\hat a$:
$$
\frac{d\vec a}{dt}=a\frac{d\hat a}{dt}+\frac{da}{dt}\cdot\hat a\\
\frac{D\vec a}{Dt}=a\frac{D\hat a}{Dt}+\frac{Da}{Dt}\cdot\hat a\\
$$
又有:
$$
\frac{d\vec a}{dt}=\frac{D\vec a}{Dt}
$$
两式相减得:
$$
\begin{aligned}
\frac{D\vec a}{Dt}-\frac{d\vec a}{dt}&=a(\frac{D\hat a}{Dt}-\frac{d\hat a}{dt})\\
&=a(\vec\omega-\vec{\omega'})\times\hat a
\end{aligned}
$$
又有:
$$
\vec\theta=\vec\theta_0+\vec\theta'
$$
即
$$
\begin{aligned}
\frac{D\vec\theta}{Dt}&=\frac{D\vec{\theta_0}}{Dt}+\frac{D\vec{\theta'}}{Dt}\\
&=\vec{\omega_0}+\frac{D(\theta\cdot\hat\theta)}{Dt}
\end{aligned}
$$
对$S,S'$来说,$\hat\theta$相同且不变,故
$$
\vec\omega=\vec{\omega_0}+\vec{\omega'}
$$
故:
$$
\frac{D\vec a}{Dt}-\frac{d\vec a}{dt}=a\vec{\omega_0}\times\hat a=\vec{\omega_0}\times\vec a
$$
由于$\vec r=\vec{r'}$
$$
\frac{D\vec r}{Dt}=\frac{D\vec{r'}}{Dt}=\frac{d\vec{r'}}{dt}+\vec{\omega_0}\times \vec{r'}
$$
即
$$
\vec v=\vec{v'}+\vec{\omega_0}\times\vec{r'}
$$
故
$$
\begin{aligned}
\vec a=\frac{D\vec v}{Dt}&=\frac D{Dt}(\vec{v'}+\vec{\omega_0}\times\vec{r'})\\
&=\frac{d\vec{v'}}{dt}+\vec{\omega_0}\times\vec{v'}+\frac{D\vec{\omega_0}}{Dt}\times\vec{r'}+\vec{\omega_0}\times(\frac{d\vec{r'}}{dt}+\vec{\omega_0}\times\vec{r'})\\
&=\vec{a'}+2\vec{\omega_0}\times\vec{v'}+\vec\alpha\times\vec{r'}+\vec{\omega_0}\times(\vec{\omega_0}\times\vec{r'})
\end{aligned}
$$
